code/experimental/P256/Hacl.Spec.P256.Normalisation.fst
@@ -5,29 +5,10 @@ open Lib.Buffer
 
 open Hacl.Spec.P256.Definitions
 open Hacl.Spec.P256.MontgomeryMultiplication
+open Hacl.Spec.P256
+open Hacl.Spec.P256.Lemmas
 
 open FStar.Math.Lemmas
- 
-let modp_inv2_pow (x: nat) : Tot (r: nat {r < prime}) = 
-   power_distributivity x (prime - 2) prime;
-   pow x (prime - 2) % prime
-
-
-let _norm (p : nat * nat * nat) =
-  let open FStar.Mul in 
-  let (x, y, z) = p in
-  let z2 = z * z in 
-  let z2i = modp_inv2_pow z2 in 
-  let z3 = z * z * z in 
-  let z3i = modp_inv2_pow z3 in 
-  let x3 = (z2i * x) % prime in 
-  let y3 = (z3i * y) % prime in 
-  let z3 = 1 in 
-  assert(x3 == (x * (pow (z * z) (prime -2) % prime) % prime));
-  assert(y3 == (y * (pow (z * z * z) (prime - 2) % prime) % prime));
-  assert(z3 == 1);
-  (x3, y3, z3)
-
 
 open FStar.Mul  
 #reset-options "--z3refresh --z3rlimit 300" 
